Add "authorization code flow" example.
Notable SVX2 framework changes:
- Support for "direct responses" (a.k.a. server-to-server calls).
- When the input and output messages of a side computation are passed (in
  that order) to an SVX method, automatically discover the relationship
  instead of treating them as independent.
- When a secret is verified, assume the parameters are equal to the ones
  from which it was originally generated.  (Currently reference equals,
  which is very unsound.  Fix it later.)

SVAuth/Main.cs
@@ -26,7 +26,8 @@ namespace SVAuth
             //RunServer();
             //SVX2_Test_Concat.Test();
             //SVX2_Test_Secret.Test();
-            SVX2_Test_ImplicitFlow.Test();
+            //SVX2_Test_ImplicitFlow.Test();
+            SVX2_Test_AuthorizationCodeFlow.Test();
 
             /* When the program is run under the debugger in Visual Studio, the
              * output window closes immediately when the program exits.  Emulate
