SVAuth/SVX2_Test_AuthorizationCodeFlow.cs
@@ -1,0 +1,371 @@
+﻿using System;
+using System.Collections.Generic;
+using System.Diagnostics.Contracts;
+using System.Linq;
+using System.Threading.Tasks;
+using SVX2;
+using System.Text.RegularExpressions;
+using Newtonsoft.Json;
+
+namespace SVAuth
+{
+    public static class SVX2_Test_AuthorizationCodeFlow
+    {
+        static readonly Principal googlePrincipal = Principal.Of("Google");
+        static readonly Principal mattMerchantPrincipal = Principal.Of("MattMerchant");
+
+        static Principal GoogleUserPrincipal(string googleUsername)
+        {
+            return Principal.Of("Google:" + googleUsername);
+        }
+
+        // Accessibility constraint on RawGenerate that doesn't seem to make sense in this case.
+        public class AuthorizationCodeParams
+        {
+            // Corresponds to GoogleUserPrincipal(username)
+            public string googleUsername;
+            public Principal rpPrincipal;
+        }
+
+        public class GoogleAuthorizationCodeGenerator : SecretGenerator<AuthorizationCodeParams>
+        {
+            protected override PrincipalHandle[] GetReaders(object theParams)
+            {
+                var params2 = (AuthorizationCodeParams)theParams;
+                return new Principal[] {
+                    // Comment this to get an internal error during secret generation.
+                    googlePrincipal,
+                    // Comment either of these to see the secret export check fail.
+                    params2.rpPrincipal,
+                    GoogleUserPrincipal(params2.googleUsername),
+                    // Uncomment to see the verification fail.
+                    //Principal.Of("other")
+                };
+            }
+
+            protected override string RawGenerate(AuthorizationCodeParams theParams)
+            {
+                // Nothing actually secret. :)
+                return JsonConvert.SerializeObject(theParams);
+            }
+
+            protected override void RawVerify(AuthorizationCodeParams theParams, string secretValue)
+            {
+                if (secretValue != RawGenerate(theParams))
+                    throw new ArgumentException();
+            }
+        }
+
+        static MessageStructure<AuthorizationCodeRequest> authorizationCodeRequestStructure;
+        static MessageStructure<AuthorizationCodeResponse> authorizationCodeResponseStructure;
+
+        static MessageStructure<ValidationRequest> validationRequestStructure;
+        static MessageStructure<ValidationResponse> validationResponseStructure;
+
+        public class AuthorizationCodeRequest : SVX_MSG
+        {
+            public Principal rpPrincipal;
+            public Secret state;
+        }
+        public class AuthorizationCodeResponse : SVX_MSG
+        {
+            public Secret authorizationCode;
+            public Secret state;
+        }
+        public class ValidationRequest : SVX_MSG
+        {
+            public Principal rpPrincipal;
+            public Secret authorizationCode;
+        }
+        public class ValidationResponse : SVX_MSG
+        {
+            public string googleUsername;
+        }
+
+        public class IdPAuthenticationEntry : SVX_MSG
+        {
+            public PrincipalHandle authenticatedClient;
+            public string googleUsername;
+        }
+        // This is an SVX_MSG just so it can be passed to an SVX method as a
+        // nondet argument.  If we add support for untracked arguments, we can
+        // just pass theParams by itself.
+        public class AuthorizationCodeParamsMessage : SVX_MSG
+        {
+            public AuthorizationCodeParams theParams;
+        }
+        public class RPAuthenticationConclusion : SVX_MSG
+        {
+            public PrincipalHandle authenticatedClient;
+            public string googleUsername;
+        }
+
+        public class Google_IdP : Participant
+        {
+            public Principal SVXPrincipal => googlePrincipal;
+            private GoogleAuthorizationCodeGenerator authorizationCodeGenerator = new GoogleAuthorizationCodeGenerator();
+
+            private Dictionary<Secret, AuthorizationCodeParams> authorizationCodeParamsDict = new Dictionary<Secret, AuthorizationCodeParams>();
+
+            public string CodeEndpoint(PrincipalHandle client, string codeRequestStr)
+            {
+                var req = JsonConvert.DeserializeObject<AuthorizationCodeRequest>(codeRequestStr);
+                authorizationCodeRequestStructure.Import(req,
+                    // We don't know who produced the request.
+                    PrincipalFacet.GenerateNew(SVXPrincipal),
+                    client);
+
+                // In reality, AuthenticateClient couldn't be done
+                // synchronously, so both TokenEndpoint and AuthenticateClient
+                // would be broken into a start and a callback.
+                var idpConc = AuthenticateClient(client);
+
+                var resp = SVX_Ops.Call(SVX_MakeAuthorizationCodeResponse, req, idpConc);
+
+                authorizationCodeParamsDict[resp.authorizationCode] = new AuthorizationCodeParams
+                {
+                    rpPrincipal = req.rpPrincipal,
+                    googleUsername = idpConc.googleUsername
+                };
+
+                authorizationCodeResponseStructure.Export(resp, client, req.rpPrincipal);
+                return JsonConvert.SerializeObject(resp);
+            }
+
+            IdPAuthenticationEntry AuthenticateClient(PrincipalHandle client)
+            {
+                // In reality, once the user logs in, we would store the
+                // IdPAuthenticationEntry in the session data structure of the
+                // web application framework.
+                var username = "Alice";
+                return SVX_Ops.Call(SVX_ConcludeClientAuthentication, new IdPAuthenticationEntry {
+                    authenticatedClient = client,
+                    googleUsername = username,
+                });
+            }
+
+            public IdPAuthenticationEntry SVX_ConcludeClientAuthentication(IdPAuthenticationEntry entry)
+            {
+                // TODO: Declare IdpSignedIn predicate here (or add to a dictionary).
+                VProgram_API.AssumeActsFor(entry.authenticatedClient, GoogleUserPrincipal(entry.googleUsername));
+                // Reuse the message... Should be able to get away with it.
+                return entry;
+            }
+
+            public AuthorizationCodeResponse SVX_MakeAuthorizationCodeResponse(AuthorizationCodeRequest req, IdPAuthenticationEntry idpConc)
+            {
+                // With this expression inlined below, BCT silently mistranslated the code.
+                var theParams = new AuthorizationCodeParams
+                {
+                    rpPrincipal = req.rpPrincipal,
+                    googleUsername = idpConc.googleUsername
+                };
+                var authorizationCode = authorizationCodeGenerator.Generate(theParams, googlePrincipal);
+
+                return new AuthorizationCodeResponse
+                {
+                    authorizationCode = authorizationCode,
+                    state = req.state
+                };
+            }
+
+            public string ValidationEndpoint(string validationRequestStr)
+            {
+                PrincipalHandle client = PrincipalFacet.GenerateNew(googlePrincipal);
+
+                var req = JsonConvert.DeserializeObject<ValidationRequest>(validationRequestStr);
+                validationRequestStructure.Import(req,
+                    // Assume validation requests are not XSRF-able.
+                    // TODO: Think more carefully about this.
+                    client,
+                    client);
+
+                var paramsMsg = new AuthorizationCodeParamsMessage
+                {
+                    theParams = authorizationCodeParamsDict[req.authorizationCode]
+                };
+
+                var resp = SVX_Ops.Call(SVX_MakeValidationResponse, req, paramsMsg);
+
+                validationResponseStructure.ExportDirectResponse(resp, client);
+                return JsonConvert.SerializeObject(resp);
+            }
+
+            public ValidationResponse SVX_MakeValidationResponse(ValidationRequest req, AuthorizationCodeParamsMessage paramsMsg)
+            {
+                // As long as we're using the interim implementation of
+                // AssumeValidSecret that assumes the parameters of equal
+                // secrets are reference equal, it's critical that we don't do
+                // anything that will introduce a contradiction.  With theParams
+                // as nondet, we should be OK for now.
+                var theParams = paramsMsg.theParams;
+                // Comment out these 2 lines to see the verification fail.
+                if (theParams.rpPrincipal != req.rpPrincipal)
+                    throw new Exception("Authorization code RP mismatch");
+                authorizationCodeGenerator.Verify(theParams, req.authorizationCode);
+                return new ValidationResponse
+                {
+                    googleUsername = theParams.googleUsername
+                };
+            }
+        }
+
+        class StateParams
+        {
+            internal string sessionId;
+        }
+        class MattMerchant_Google_StateGenerator : SecretGenerator<StateParams>
+        {
+            protected override PrincipalHandle[] GetReaders(object theParams)
+            {
+                var params2 = (StateParams)theParams;
+                return new PrincipalHandle[] { googlePrincipal, mattMerchantPrincipal,
+                    PrincipalFacet.Of(mattMerchantPrincipal, params2.sessionId) };
+            }
+
+            protected override string RawGenerate(StateParams theParams)
+            {
+                return "mattmerchant_google_state:" + theParams.sessionId;
+            }
+
+            protected override void RawVerify(StateParams theParams, string secretValue)
+            {
+                if (secretValue != RawGenerate(theParams))
+                    throw new ArgumentException();
+            }
+        }
+
+        public class MattMerchant_RP : Participant
+        {
+            // XXX Definitely needs to be a parameter.
+            public Principal SVXPrincipal => mattMerchantPrincipal;
+
+            MattMerchant_Google_StateGenerator stateGenerator = new MattMerchant_Google_StateGenerator();
+
+            public string LoginStart(PrincipalHandle client)
+            {
+                var req = new AuthorizationCodeRequest
+                {
+                    rpPrincipal = SVXPrincipal,
+                    // XXX This cast is a little contrived.  Decide if we want
+                    // to pass the client as a session ID or a facet or what.
+                    state = stateGenerator.Generate(
+                        new StateParams { sessionId = ((PrincipalFacet)client).id },
+                        SVXPrincipal)
+                };
+                authorizationCodeRequestStructure.Export(req, client, googlePrincipal);
+                return JsonConvert.SerializeObject(req);
+            }
+
+            public void LoginCallback(PrincipalHandle client, string idTokenResponseStr, Google_IdP idp)
+            {
+                var authorizationCodeResponse = JsonConvert.DeserializeObject<AuthorizationCodeResponse>(idTokenResponseStr);
+                authorizationCodeResponseStructure.Import(authorizationCodeResponse,
+                    // We don't know who produced the redirection.
+                    PrincipalFacet.GenerateNew(SVXPrincipal),
+                    client);
+
+                var validationRequest = SVX_Ops.Call(SVX_MakeValidationRequest, authorizationCodeResponse);
+
+                validationRequestStructure.Export(validationRequest, googlePrincipal, null);
+                var validationRequestStr = JsonConvert.SerializeObject(validationRequest);
+
+                var validationResponseStr = idp.ValidationEndpoint(validationRequestStr);
+
+                var validationResponse = JsonConvert.DeserializeObject<ValidationResponse>(validationResponseStr);
+                validationResponseStructure.ImportDirectResponse(validationResponse, googlePrincipal, SVXPrincipal);
+
+                // SVX will automatically detect using message IDs that
+                // validationResponse actually resulted from
+                // authorizationCodeResponse and not merely another message with
+                // the same SymT.  This is essential for us to establish the
+                // relationship between authorizationCodeResponse.SVX_sender and
+                // validationResponse.googleUsername.
+                var conc = SVX_Ops.Call(SVX_SignInRP, authorizationCodeResponse, validationResponse);
+
+                SVX_Ops.Certify(conc, LoginSafety, new Principal[] { googlePrincipal, SVXPrincipal });
+                //SVX_Ops.Certify(conc, LoginXSRFPrevention, new Principal[] { });
+                // AbandonAndCreateSession...
+            }
+
+            public ValidationRequest SVX_MakeValidationRequest(AuthorizationCodeResponse resp)
+            {
+                return new ValidationRequest
+                {
+                    authorizationCode = resp.authorizationCode,
+                    rpPrincipal = SVXPrincipal  // Like in the original authorization code request.
+                };
+            }
+
+            public RPAuthenticationConclusion SVX_SignInRP(
+                AuthorizationCodeResponse authorizationCodeResponse, ValidationResponse validationResponse)
+            {
+                return new RPAuthenticationConclusion {
+                    authenticatedClient = authorizationCodeResponse.SVX_sender,
+                    googleUsername = validationResponse.googleUsername
+                };
+            }
+
+            public static bool LoginSafety(RPAuthenticationConclusion conc)
+            {
+                var targets = new PrincipalHandle[3];
+                targets[0] = googlePrincipal;
+                targets[1] = mattMerchantPrincipal;
+                targets[2] = GoogleUserPrincipal(conc.googleUsername);
+                return VProgram_API.ActsForAny(conc.authenticatedClient, targets);
+            }
+
+            public static bool LoginXSRFPrevention(RPAuthenticationConclusion conc)
+            {
+                // TODO
+#if false
+                var targets = new PrincipalHandle[3];
+                targets[0] = googlePrincipal;
+                targets[1] = mattMerchantPrincipal;
+                targets[2] = GoogleUserPrincipal(conc.googleUsername);
+                return VProgram_API.ActsForAny(conc.authenticatedClient, targets);
+#endif
+                throw new NotImplementedException();
+            }
+        }
+
+        [BCTOmitImplementation]
+        static SVX2_Test_AuthorizationCodeFlow()
+        {
+            // In all cases, we only bother declaring the secret readers we
+            // actually need for the protocol flow.  Maybe this is a bad habit.
+
+            authorizationCodeRequestStructure = new MessageStructure<AuthorizationCodeRequest>();
+            authorizationCodeRequestStructure.AddSecret(nameof(AuthorizationCodeRequest.state),
+                // The sender (the client) gets implicitly added.
+                (msg) => new PrincipalHandle[] { msg.rpPrincipal });
+
+            authorizationCodeResponseStructure = new MessageStructure<AuthorizationCodeResponse>();
+            authorizationCodeResponseStructure.AddSecret(nameof(AuthorizationCodeRequest.state),
+                (msg) => new PrincipalHandle[] { });
+            authorizationCodeResponseStructure.AddSecret(nameof(AuthorizationCodeResponse.authorizationCode),
+                (msg) => new PrincipalHandle[] { googlePrincipal });
+
+            validationRequestStructure = new MessageStructure<ValidationRequest>();
+            validationRequestStructure.AddSecret(nameof(AuthorizationCodeResponse.authorizationCode),
+                (msg) => new PrincipalHandle[] { });
+
+            // Nothing interesting here.
+            validationResponseStructure = new MessageStructure<ValidationResponse>();
+        }
+
+        [BCTOmitImplementation]
+        public static void Test()
+        {
+            var idp = new Google_IdP();
+            var rp = new MattMerchant_RP();
+
+            var aliceIdP = PrincipalFacet.GenerateNew(googlePrincipal);
+            var aliceRP = PrincipalFacet.GenerateNew(mattMerchantPrincipal);
+
+            var codeRequestStr = rp.LoginStart(aliceRP);
+            var codeResponseStr = idp.CodeEndpoint(aliceIdP, codeRequestStr);
+            rp.LoginCallback(aliceRP, codeResponseStr, idp);  // Includes the validation server-to-server call
+        }
+    }
+}
