SVX_Ops/SVX2/SymT.cs
@@ -29,10 +29,20 @@ namespace SVX2
     }
     abstract class SymT
     {
-        // TODO
+        // Generate a fresh one by default.  This will just be wasted work and
+        // get overwritten when deserializing.
+        internal string messageId = Utils.RandomIdString();
+
         internal abstract string MessageTypeFullName { get; }
         internal abstract IEnumerable<SymT> EmbeddedSymTs { get; }
+        // This only goes one level down.  It means the caller has to do the
+        // recursion, but also means the caller has control of the recursion
+        // (e.g., whether it happens before or after rewriting the root, both,
+        // or neither in certain cases) without us having to provide multiple
+        // variants of this method.
+        internal abstract SymT RewriteEmbeddedSymTs(Func<SymT, SymT> rewriter);
     }
+
     [JsonObject(MemberSerialization.Fields)]
     class SymTNondet : SymT
     {
@@ -40,7 +50,9 @@ namespace SVX2
 
         internal override string MessageTypeFullName => messageTypeFullName;
         internal override IEnumerable<SymT> EmbeddedSymTs => new SymT[] { };
+        internal override SymT RewriteEmbeddedSymTs(Func<SymT, SymT> rewriter) => this;
     }
+
     [JsonObject(MemberSerialization.Fields)]
     class SymTMethod : SymT
     {
@@ -53,7 +65,18 @@ namespace SVX2
 
         internal override string MessageTypeFullName => methodReturnTypeFullName;
         internal override IEnumerable<SymT> EmbeddedSymTs => inputSymTs;
+        internal override SymT RewriteEmbeddedSymTs(Func<SymT, SymT> rewriter) =>
+            new SymTMethod
+            {
+                messageId = messageId,
+                participantId = participantId,
+                methodName = methodName,
+                methodReturnTypeFullName = methodReturnTypeFullName,
+                methodArgTypeFullNames = methodArgTypeFullNames,
+                inputSymTs = inputSymTs.Select(rewriter).ToArray()
+            };
     }
+
     class VerifyOnImportEntry
     {
         internal string fieldPath;
@@ -66,6 +89,7 @@ namespace SVX2
         internal SymTTransfer(SymTTransfer copyFrom)
         {
             // XXX Aliasing
+            messageId = copyFrom.messageId;
             originalSymT = copyFrom.originalSymT;
             hasSender = copyFrom.hasSender;
             producer = copyFrom.producer;
@@ -78,9 +102,12 @@ namespace SVX2
         internal SymT originalSymT;
 
         internal bool hasSender;
-        // These are non-null if recorded concretely.  Currently, we record all
-        // principals and no facets, so avoid a cast in the emit.
-        internal Principal producer, sender;
+
+        // In general, the producer should be filled in even if it is a facet,
+        // in case it is a direct client that we're going to replace.  Let's do
+        // the same for the sender to maintain consistency.  Facets get erased
+        // when we actually prepare a CertificationRequest.
+        internal PrincipalHandle producer, sender;
 
         // This one is a list so we can mutate it little by little during import. :/
         internal List<VerifyOnImportEntry> payloadSecretsVerifiedOnImport = new List<VerifyOnImportEntry>();
@@ -90,8 +117,21 @@ namespace SVX2
         internal SymT fallback;
 
         internal override string MessageTypeFullName => originalSymT.MessageTypeFullName;
-        internal override IEnumerable<SymT> EmbeddedSymTs => new SymT[] { originalSymT };
+        internal override IEnumerable<SymT> EmbeddedSymTs =>
+            fallback == null ? new SymT[] { originalSymT } : new SymT[] { originalSymT, fallback };
+        internal override SymT RewriteEmbeddedSymTs(Func<SymT, SymT> rewriter) =>
+            new SymTTransfer
+            {
+                messageId = messageId,
+                originalSymT = rewriter(originalSymT),
+                hasSender = hasSender,
+                producer = producer,
+                sender = sender,
+                payloadSecretsVerifiedOnImport = payloadSecretsVerifiedOnImport,
+                fallback = (fallback == null) ? null : rewriter(fallback),
+            };
     }
+
     [JsonObject(MemberSerialization.Fields)]
     class NestedSymTEntry
     {
@@ -106,8 +146,30 @@ namespace SVX2
 
         internal override string MessageTypeFullName => rootSymT.MessageTypeFullName;
 
+        // SymTComposite shares the messageId of its rootSymT.  It's unfortunate
+        // that the messageId gets redundantly serialized, but not worth
+        // complicating things to avoid.  This setter lets us continue to use
+        // the object initializer syntax.
+        internal SymT RootSymTWithMessageId
+        {
+            set
+            {
+                rootSymT = value;
+                messageId = rootSymT.messageId;
+            }
+        }
+
         internal override IEnumerable<SymT> EmbeddedSymTs =>
             new SymT[] { rootSymT }.Concat(nestedSymTs.Select((e) => e.symT));
+        internal override SymT RewriteEmbeddedSymTs(Func<SymT, SymT> rewriter) =>
+            new SymTComposite
+            {
+                RootSymTWithMessageId = rewriter(rootSymT),
+                nestedSymTs = nestedSymTs.Select((entry) => new NestedSymTEntry {
+                    fieldPath = entry.fieldPath,
+                    symT = rewriter(entry.symT)
+                }).ToArray()
+            };
     }
 
     // We don't actually serialize this yet, but we will once we have the
